src/PartialMonotonicity.v
@@ -2,24 +2,30 @@
 (* Clément Blaudeau - LAMP@EPFL 2021 *)
 (** This file defines the notion of partial monotonicity between stores. The idea behind partial monotonicity is simple: objects that are being initialized (not warm already) can only get "warmer": the number of initialized fields can only increase. Between two stores [σ] and [σ'], it means that all objects in [σ] have more initialized fields in [σ']; it does not states anything about new objects that [σ'] can have. *)
 
-From Celsius Require Export Compatibility.
+From Celsius Require Export Compatibility Reachability.
 Require Import ssreflect ssrbool List Psatz Coq.Program.Tactics.
 Import ListNotations.
 Open Scope nat_scope.
 
 (** ** Definitions and notations *)
-Definition initializedFields σ l (f: list Field) : Prop :=
+Definition initialized_fields σ l (f: list Field) : Prop :=
   match (getObj σ l) with
   | Some (C, ω) => ((length f) <= (length ω))
   | _ => False
   end.
-Notation "σ ⊨ l : f" := (initializedFields σ l f) (at level 80, l at level 98, f at level 98).
 
-Definition partialMonotonicity σ σ' :=
+Global Instance notation_initialized_fields : notation_dash_colon Store Loc (list Field) :=
+  { dash_colon_ := initialized_fields }.
+Global Hint Unfold notation_initialized_fields: notations.
+
+Definition partial_monotonicity σ σ' :=
   forall l f, (σ ⊨ l : f) -> (σ' ⊨ l : f).
-Notation "σ ⪯ σ'" := (partialMonotonicity σ σ') (at level 0).
-#[global] Hint Unfold partialMonotonicity: pM.
 
+Notation "s ⪯ s'" := (partial_monotonicity s s') (at level 60).
+
+Local Hint Unfold partial_monotonicity: pM.
+Local Hint Unfold initialized_fields: pM.
+Implicit Type σ: Store.
 
 (** ** Basic results *)
 (** The relation is trivially reflexive *)
@@ -28,7 +34,7 @@ Lemma pM_refl: forall σ,
 Proof.
   auto with pM.
 Qed.
-#[global] Hint Resolve pM_refl: pM.
+Global Hint Resolve pM_refl: pM.
 
 (** The relation is trivially transitive *)
 Lemma pM_trans : forall σ1 σ2 σ3,
@@ -36,9 +42,9 @@ Lemma pM_trans : forall σ1 σ2 σ3,
     σ2 ⪯ σ3 ->
     σ1 ⪯ σ3.
 Proof.
-  auto with pM.
+  autounfold with notations. eauto with pM.
 Qed.
-#[global] Hint Resolve pM_trans: pM.
+Global Hint Resolve pM_trans: pM.
 
 Ltac pM_trans :=
   repeat match goal with
@@ -46,41 +52,43 @@ Ltac pM_trans :=
          | H: ?σ1 ⪯ ?σ2 |- ?σ1 ⪯ ?σ3 => apply pM_trans with σ2 ; [ assumption | ]
          | H: ?σ2 ⪯ ?σ3 |- ?σ1 ⪯ ?σ3 => apply pM_trans with σ2 ; [ | assumption ]
          end.
-#[global] Hint Extern 1 => pM_trans: pM.
+Global Hint Extern 1 => pM_trans: pM.
 
 
 (** Initialized fields are within the domain *)
-Lemma initializedFields_dom :
+Lemma initialized_fields_dom :
   forall σ l f,
     (σ ⊨ l : f) -> (l < (dom σ)).
 Proof.
-  unfold initializedFields, getObj.
+  autounfold with notations.
+  unfold initialized_fields, getObj.
   induction σ; destruct l as [| l']; steps; try lia.
   eapply Le.le_n_S, IHσ; rewrite_any; eauto.
 Qed.
-Global Hint Resolve initializedFields_dom: pM.
+Global Hint Resolve initialized_fields_dom: pM.
 
 (** Technical result: an object always have 0 or more fields initialized *)
-Lemma initializedFields_exists :
-  forall σ c e,
-  exists f, ((c,e)::σ) ⊨ (dom σ) : f.
+Lemma initialized_fields_exists :
+  forall σ C ω,
+  exists f, ((C,ω)::σ) ⊨ (dom σ) : f.
 Proof.
-  unfold initializedFields.
+  autounfold with notations pM core.
+  unfold initialized_fields.
   intros. exists ([]: list Field).
   induction σ; intros ; simpl ; try lia.
-  - destruct σ, a; steps; lia.
+  destruct σ, a; steps; lia.
 Qed.
-Global Hint Resolve initializedFields_exists: pM.
+Global Hint Resolve initialized_fields_exists: pM.
 
 (** We have a result on the store sizes *)
 Lemma pM_domains:
   forall σ σ',
     σ ⪯ σ' -> dom σ <= dom σ'.
 Proof.
-  unfold partialMonotonicity; intros.
+  autounfold; unfold partial_monotonicity; intros.
   destruct σ eqn:Σ; simpl; [lia |].
   destruct o.
-  case : (initializedFields_exists l c e) => f Hf.
+  move : (initialized_fields_exists s c e) => [f Hf].
   eauto using Lt.lt_le_S with pM.
 Qed.
 Global Hint Resolve pM_domains: pM.
@@ -89,12 +97,12 @@ Global Hint Resolve pM_domains: pM.
 (** ** Main Monotonicity result *)
 (** We start with two technical results on partial monotonicity for assignment (update) and fresh location *)
 Lemma pM_assignment :
-  forall σ l C ω ω',
+  forall σ l C (ω ω': Env),
     getObj σ l = Some (C, ω) ->
     length ω <= length ω' ->
     σ ⪯ [l ↦ (C, ω')]σ.
 Proof.
-  unfold partialMonotonicity, initializedFields.
+  autounfold with pM notations.
   intros.
   destruct_eq (l = l0); subst;
     repeat rewrite_any;
@@ -107,22 +115,25 @@ Lemma pM_freshness :
   forall σ c ρ,
     σ ⪯ (σ ++ [(c, ρ)]).
 Proof.
-  unfold partialMonotonicity, initializedFields.
-  induction σ ; destruct l => //.
-  apply IHσ => //.
+  autounfold with notations pM. unfold getObj.
+  steps;
+    rewrite nth_error_app1 in matched; steps;
+    apply nth_error_Some; steps.
 Qed.
 Global Hint Resolve pM_freshness: pM.
 
 (** Then we have the main result *)
 Theorem pM_theorem:
   forall e σ σ' ρ ψ v,
-      ⟦e⟧p (σ, ρ, ψ) --> (v, σ') -> σ ⪯ σ'.
+      ⟦e⟧ (σ, ρ, ψ) --> (v, σ') -> σ ⪯ σ'.
 Proof with (eauto with pM updates lia).
   intros.
   induction H using evalP_ind2 with
     (Pl := fun _ σ _ _ _ σ' _ => σ ⪯ σ')
     (Pin := fun _ _ _ σ σ' _ => σ ⪯ σ');
-    unfold assign, assign_new in *; steps; pM_trans ...
+    unfold assign, assign_new in *;
+    repeat destruct_match;
+    flatten; pM_trans ...
 Qed.
 Global Hint Resolve pM_theorem: pM.
 
@@ -141,8 +152,8 @@ Theorem pM_theorem_init:
 Proof with (eauto with pM updates lia).
   intros.
   induction H;
-    unfold assign, assign_new in *; steps ...
-  eapply pM_theorem in H. pM_trans ...
+    unfold assign, assign_new in *; ground ...
+  eapply pM_theorem in H ...
 Qed.
 Global Hint Resolve pM_theorem_init: pM.
 
@@ -187,14 +198,15 @@ Ltac eval_dom :=
 
 
 (** If we combine partial monotonicity with compatibility (objects do no change type), we can prove that warm objects stay warm *)
-Lemma partialMonotonicity_warm_monotone:
-  forall σ σ' l,
+Lemma pM_warm_monotone:
+  forall σ σ' (l: Loc),
     σ ⪯ σ' ->
-    σ ⊆ σ' ->
-    (σ ⊨ l : warm) ->
-    (σ' ⊨ l : warm).
+    σ ⪨ σ' ->
+    σ  ⊨ l : warm ->
+    σ' ⊨ l : warm.
 Proof.
-  unfold partialMonotonicity, initializedFields, reachable_warm; steps.
+  autounfold with pM core notations. unfold reachable_warm.
+  steps.
   specialize (H l fields).
   repeat rewrite_any.
   eapply H0 in H2; steps.
