src/Scopability.v
@@ -3,25 +3,20 @@
 (** This file defines the notions of scoping and scoping preservation. There are more complex and subtle, and should not serve as an introduction to the local reasonning properties.
 The main idea is pretty natural: to ensure that newly created objects are hot, we need to check that, transitively, all locations reachable from the attributes of the object are intialized. To do so, we need to be able to reason about the set of locations that are reachable from a set of attributes in a given store. Given two stores [σ] and [σ'], and two sets of locations [L] and [L'], the pair [(σ, L)] "scopes" [(σ',L')] if all locations reachable from [L'] in [σ'] were already reachable from [L] in [σ].
  But as we allow to manipulate objects under initialization, we also need to consider a notion of "preservation" : scoping relations that are maintained when updating from one store to another. *)
-
 From Celsius Require Export PartialMonotonicity Compatibility Wellformedness Reachability Tactics.
 Require Import ssreflect ssrbool Psatz Sets.Ensembles List.
 Import ListNotations.
 Open Scope nat_scope.
-
 (** ** Definitions and Notations *)
 (* The scoping relation, with the hypothesis that the sets of locations are "correct" (within the stores) *)
 Definition scoping (σ σ': Store) (L L': Ensemble Loc) :=
   L ⪽ σ ->
   L' ⪽ σ' ->
-  (forall l, l < dom σ -> (σ' ⊫ L' ⇝ l) -> σ ⊫ L ⇝ l).
-
+  (forall (l:Loc), l < dom σ -> (σ' ⊨ L' ⇝ l) -> σ ⊨ L ⇝ l).
 Notation "( σ1 , L1 )  ⋖  ( σ2 , L2 )" := (scoping σ1 σ2 L1 L2) (at level 0).
-Notation "( σ1 , { l } )  ⋖  ( σ2 , L2 )" := (scoping σ1 σ2 {l} L2) (at level 0).
-Notation "( σ1 , L1 )  ⋖  ( σ2 , { l } )" := (scoping σ1 σ2 L1 {l}) (at level 0).
-Notation "( σ1 , { l1 } )  ⋖  ( σ2 , { l2 } )" := (scoping σ1 σ2 {l1} {l2}) (at level 0).
-
-
+Notation "( σ1 ,  { l } )  ⋖  ( σ2 , L2 )" := (scoping σ1 σ2 {l} L2) (at level 0).
+Notation "( σ1 , L1 )  ⋖  ( σ2 ,  { l } )" := (scoping σ1 σ2 L1 {l}) (at level 0).
+Notation "( σ1 ,  { l1 } )  ⋖  ( σ2 ,  { l2 } )" := (scoping σ1 σ2 {l1} {l2}) (at level 0).
 (* The scoping preservation, with technical choices of hypothesis: *)
 Definition scoping_preservation (σ1 σ2: Store) (L: LocSet) :=
   (L ⪽ σ1) /\
@@ -34,88 +29,81 @@ Definition scoping_preservation (σ1 σ2: Store) (L: LocSet) :=
     (σ0, L0) ⋖ (σ1, L1) ->
     (σ0, L0) ⋖ (σ2, L1).
 Notation "σ1 ⇝ σ2 ⋖ L" := (scoping_preservation σ1 σ2 L) (at level 99).
-
-Global Hint Unfold scoping : scp.
-Global Hint Unfold scoping_preservation : scp.
+Local Hint Unfold scoping : scp.
+Local Hint Unfold scoping_preservation : scp.
 Global Hint Unfold reachability_set: scp.
 Global Hint Resolve Union_introl: scp.
 Global Hint Resolve Union_intror: scp.
 
-
 (** ** Basic results *)
 (** We first show a set of basic results about scoping. The premisses can sometime look a bit arbitrary, but they are actually fine-tuned *)
-
 Lemma scp_refl :
   forall σ L, (σ, L) ⋖ (σ, L).
 Proof.
   eauto with scp.
 Qed.
 Global Hint Resolve scp_refl: scp.
-
 Lemma scp_refl2 :
   forall σ L1 L2, L2 ⊆ L1 -> (σ, L1) ⋖ (σ, L2).
 Proof.
-  unfold scoping, reachability_set; steps.
-  exists l'; steps; eapply H => //.
+  unfold scoping. steps; rch_set.
+  exists l0; steps; eapply H => //.
 Qed.
 Global Hint Resolve scp_refl2: scp.
-
 Lemma scp_subset :
   forall σ1 σ2 L L1 L2,
     (σ1, L1) ⋖ (σ2, L2) ->
     L ⊆ L2 ->
     L2 ⪽ σ2  ->
     (σ1, L1) ⋖ (σ2, L).
-Proof with (eauto with scp).
-  unfold scoping, reachability_set; steps ...
+Proof with (eauto with scp lia).
+  unfold scoping; steps ...
+  apply H ...
+  rch_set.
+  exists l0; steps ...
 Qed.
 Global Hint Resolve scp_subset: scp.
-
 Lemma scp_union :
   forall σ1 σ2 L L1 L2,
     (σ1, L)  ⋖ (σ2, L1) ->
     (σ1, L)  ⋖ (σ2, L2) ->
     (σ1, L)  ⋖ (σ2, L1∪L2).
 Proof.
-  unfold scoping, reachability_set; steps.
+  autounfold with notations scp. steps.
   inversion H4; steps; eauto with wf.
 Qed.
 Global Hint Resolve scp_union: scp.
-
 Lemma scp_union_introl :
   forall σ1 σ2 L L1 L2,
     (L1 ∪ L2) ⪽ σ2 ->
     (σ1, L) ⋖ (σ2, L1∪L2) ->
     (σ1, L) ⋖ (σ2, L1).
 Proof.
-  unfold scoping, reachability_set; steps.
+  autounfold with notations scp ; steps.
   eauto with scp.
 Qed.
 Global Hint Resolve scp_union_introl: scp.
-
 Lemma scp_union_intror :
   forall σ1 σ2 L L1 L2,
     (L1 ∪ L2) ⪽ σ2 ->
     (σ1, L)  ⋖ (σ2, L1∪L2) ->
     (σ1, L)  ⋖ (σ2, L2).
 Proof.
-  unfold scoping, reachability_set; steps.
+  autounfold with notations scp ; steps.
   eauto with scp.
 Qed.
 Global Hint Resolve scp_union_intror: scp.
-
 
 Lemma scp_reachability:
   forall σ l1 l2,
     σ ⊨ l1 ⇝ l2 ->
     (σ, {l1}) ⋖ (σ, {l2}).
 Proof.
-  unfold scoping, reachability_set ; steps.
-  eauto with scp.
+  autounfold with notations scp ; steps.
   exists l1; try inSingleton; steps; eauto with scp rch.
+  eapply rch_trans; eauto.
 Qed.
 Global Hint Resolve scp_reachability: scp.
-
 
 Lemma scp_trans:
   forall σ1 σ2 σ3 L1 L2 L3,
@@ -125,10 +113,9 @@ Lemma scp_trans:
     (σ2, L2) ⋖ (σ3, L3) ->
     (σ1, L1) ⋖ (σ3, L3).
 Proof with eauto with scp lia.
-  unfold scoping, reachability_set; steps...
+  autounfold with notations scp. steps...
 Qed.
 Global Hint Resolve scp_trans: scp.
-
 Lemma scp_pr_trans:
   forall σ1 σ2 σ3 L1 L2,
     σ1 ⇝ σ2 ⋖ L1 ->
@@ -143,18 +130,16 @@ Proof with (eauto with wf lia).
   eapply scp_trans with σ1 L1 ...
 Qed.
 Global Hint Resolve scp_pr_trans: scp.
-
 Lemma scp_pr_regularity_degenerate:
   forall σ1 σ2 L,
     σ1 ⇝ σ2 ⋖ L ->
     (dom σ1) <= (dom σ2) ->
     (σ1, L) ⋖ (σ2, L).
 Proof.
-  unfold scoping_preservation, scoping; simpl; steps.
+  autounfold with scp notations ; simpl; steps.
   eauto with scp.
 Qed.
 Global Hint Resolve scp_pr_regularity_degenerate: scp.
-
 Lemma scp_pr_regularity:
   forall σ0 σ1 σ2 L L1,
     σ1 ⇝ σ2 ⋖ L ->
@@ -169,7 +154,6 @@ Proof.
   unfold scoping_preservation; steps.
 Qed.
 Global Hint Resolve scp_pr_regularity: scp.
-
 Lemma scp_pr_trans_degenerate:
   forall σ1 σ2 σ3 L1 ,
     σ1 ⇝ σ2 ⋖ L1 ->
@@ -180,7 +164,6 @@ Proof.
   steps; eauto with scp.
 Qed.
 Global Hint Resolve scp_pr_trans_degenerate: scp.
-
 Lemma scp_add:
   forall σ σ' ρ' l0 l a,
     (σ, a) ⋖ (σ', {l}) ->
@@ -199,7 +182,6 @@ Proof.
       + inSingleton; apply Union_intror; steps. }
   rewrite H1; eauto with scp.
 Qed.
-
 Lemma scp_add_env:
   forall I v s c e0,
     getObj s I = Some (c, e0) ->
@@ -220,7 +202,6 @@ Proof.
     simpl; try (eexists; split); eauto with wf.
 Qed.
 Global Hint Resolve scp_add_env: scp.
-
 Lemma reachability_not_empty: forall σ C l1 l2,
     wf σ ->
     (σ++[(C, [])]) ⊨ l1 ⇝ l2 ->
@@ -235,21 +216,18 @@ Proof with (eauto with rch).
     right. steps ...
   - eapply getObj_last_empty in H1; steps ...
 Qed.
-
 Lemma reachability_add_empty: forall σ C L l,
     wf σ ->
-    (σ++[(C, [])]) ⊫ L ⇝ l ->
-    (σ ⊫ L ⇝ l) \/ l = length σ.
+    (σ++[(C, [])]) ⊨ L ⇝ l ->
+    (σ ⊨ L ⇝ l) \/ l = length σ.
 Proof.
   intros.
   inversion H0 as [l1 [Hl1 Hrch]].
   eapply reachability_not_empty in Hrch; steps.
   left. exists l1; eauto.
 Qed.
-
 (** ** Assignment results *)
 (** We prove some specific results on scopability in the context of assignment. The key reasonning technique is to do a case analysis on the presence of the modified entry in the reachability path. *)
-
 Lemma scp_assign:
   forall σ1 σ2 σ2' L1 l l' f C ω ω',
     σ1 ⇝ σ2 ⋖ L1 ->
@@ -286,7 +264,7 @@ Proof.
            assert (σ2 ⊨ l' ⇝ l0). {
              eapply reachable_path_reachability.
              eapply contains_edge_split in Hedge0 ; flatten; eauto.
-             rewrite Hedge2 in H9.
+             rewrite H10 in H9.
              eapply (reachable_path_app2 _ l' (l::p2) (l0::p1')) in H9.
              eapply reachable_path_assignment in H9; eauto.
              flatten; eauto with rch.
@@ -323,7 +301,7 @@ Proof.
            eapply reachable_path_reachability.
            destruct_eq (l' = l0); subst ; [left; split; eauto; lia | right ].
            eapply contains_edge_split in Hedge0 ; flatten; [steps | eauto].
-           rewrite Hedge2 in H7.
+           rewrite H9 in H7.
            eapply (reachable_path_app2 _ l' (l::p2) (l0::p1')) in H7.
            eapply reachable_path_assignment in H7; eauto.
            flatten; eauto with rch.
@@ -333,11 +311,9 @@ Proof.
              eauto using In_singleton with wf rch updates.
            eapply reachable_path_reachability; eauto.
 Qed.
-
 (** ** Evaluation-maintained results *)
 Global Hint Extern 1 => repeat rch_singleton: scp.
 Global Hint Extern 1 => rewrite update_dom : updates.
-
 (** ** Main Scopability theorem *)
 (** We show the main theorem. As for wellformedness theorem, we have to make a custom proof. We use the results shown for initialization, lists and assignment *)
 Theorem scopability_theorem:
@@ -345,7 +321,7 @@ Theorem scopability_theorem:
     ⟦e⟧p (σ, ρ, ψ) --> (v, σ') ->
     (codom ρ) ∪ {ψ} ⪽ σ -> wf σ ->
     ((σ, ((codom ρ) ∪ {ψ})) ⋖ (σ', {v})) /\ (σ ⇝ σ' ⋖ ((codom ρ) ∪ {ψ})) .
-Proof with (timeout 10 eauto with scp wf rch lia).
+Proof with (rch_set; timeout 10 eauto with scp wf rch lia).
   intros.
   move: H0 H1.
   induction H using evalP_ind2 with
@@ -363,13 +339,14 @@ Proof with (timeout 10 eauto with scp wf rch lia).
     unfold assign, assign_new in * ; intros; eval_dom; eval_wf;
     try solve [rch_singleton; eauto with scp lia].
   - (* e = x *)
-    unfold scoping; steps...
+    unfold scoping; steps ...
     exists l ...
   - (* e = e0.f *)
-    unfold scoping; steps; rch_singleton ...
-    assert ((σ,  (codom ρ) ∪ ({ψ})) ⋖ (σ1, {l})) as C1 by
-        (eapply scp_trans with σ1 {l1}; eauto with updates rch wf scp).
-    eapply C1 ; steps ...
+    unfold scoping; steps; rch_singleton.
+    assert ((σ,  (codom ρ) ∪ ({ψ})) ⋖ (σ1, {l})) as C1.
+    + eapply scp_trans with σ1 {l1}; eauto with wf.
+      unfold scoping; steps...
+    + eapply C1 ; steps ...
   - (* e = e0.m(l0) *)
     destruct IHevalP1, IHevalP2; eauto with wf.
     destruct IHevalP3; eauto with wf.
@@ -385,7 +362,7 @@ Proof with (timeout 10 eauto with scp wf rch lia).
     assert (dom σ1 <= dom (σ1 ++ [(C, [])])) by (rewrite dom_app; lia).
     destruct IHevalP0; eauto with wf .
     + rewrite dom_app ...
-    + eapply storeSubset_union ...
+    + eapply storeSubset_union; [eapply storeSubset_trans; eauto with lia updates |].
       eapply storeSubset_singleton3 .
       rewrite dom_app ... (* storeSubset_add_empty ? *)
     + intros ? ; steps.
@@ -396,23 +373,25 @@ Proof with (timeout 10 eauto with scp wf rch lia).
         exists l0; steps.
         eapply H_vals in H6 ...
       * inSingleton.
-        eapply reachability_not_empty in H__rch as [ ] ...
+        eapply reachability_not_empty in H__rch; steps; try lia.
         eapply reachability_dom2 in H6. lia.
     + eapply scp_pr_trans; eauto.
       unfold scoping_preservation; steps; eauto.
       unfold scoping; steps.
       move: H15 => [l0 [Hl0 H__rch]].
-      eapply reachability_not_empty in H__rch as [ ]...
+      eapply reachability_not_empty in H__rch; steps; try lia.
+      apply H11 ... exists l0 ...
     + flatten; split => //.
       eapply scp_union_intror ; eauto with wf scp.
       eapply storeSubset_union.
       eapply storeSubset_trans; eauto with wf lia.
       eapply storeSubset_trans; eauto with wf lia.
-      eapply storeSubset_singleton3 ...
+      eapply storeSubset_singleton3.
       rewrite dom_app; lia.
   - (* e = e0.f = e1; e2 *)
     destruct (getObj σ2 v1) as [[C ω] |] eqn: H__obj.
-    + destruct IHevalP1, IHevalP2 ...
+    + destruct IHevalP1; eauto.
+      destruct IHevalP2; eauto with wf lia.
       destruct IHevalP3; eauto with wf lia.
       * eapply storeSubset_trans with σ2; eauto with updates ...
       * eapply scp_assign with (f := x) (σ1 := σ) (l' := v2) (L1 := (codom ρ ∪ {ψ})) in H__obj as [ ];
@@ -423,7 +402,9 @@ Proof with (timeout 10 eauto with scp wf rch lia).
            eapply storeSubset_trans with σ2; eauto with updates wf lia.
         -- eapply scp_pr_trans; eauto with scp; update_dom ; eauto with wf lia.
            eapply_any; update_dom...
-    + destruct IHevalP1, IHevalP2, IHevalP3 ...
+    + destruct IHevalP1; eauto.
+      destruct IHevalP2; eauto with wf lia.
+      destruct IHevalP3; eauto with wf lia.
       split .
       * eapply scp_trans with (σ2 := σ2) (L2 := codom ρ ∪ {ψ}) ...
       * eapply scp_pr_trans ...
@@ -433,10 +414,14 @@ Proof with (timeout 10 eauto with scp wf rch lia).
       inversion H3; steps.
     + eapply scp_pr_trans_degenerate ...
   - (* el_cons *)
-    destruct IHevalP, IHevalP0 ...
+    destruct IHevalP; eauto.
+    destruct IHevalP0; eauto with wf lia.
     split.
     + rewrite codom_cons.
-      eapply scp_union ...
+      eapply scp_union.
+      * apply H7; eauto with lia wf.
+        apply H5; eauto.
+      * eapply scp_trans with (σ2 := σ1) (L2 := codom ρ ∪ {ψ}) ...
     + eapply scp_pr_trans_degenerate ...
   - (* init_cons *)
     destruct IHevalP; eauto.
@@ -444,8 +429,8 @@ Proof with (timeout 10 eauto with scp wf rch lia).
     inversion H__assign; subst.
     specialize (IHevalP0 L σ0).
     destruct IHevalP0; eauto with updates wf lia.
-    + eapply scp_add_env ...
-      eapply H3.
+    + eapply scp_add_env; eauto with lia wf;
+        try apply H3 ...
     + eapply scp_pr_trans; eauto.
       eapply scp_pr_trans; eauto.
       unfold scoping_preservation; intros ...
