src/Language.v
@@ -1,0 +1,68 @@
+(* Celsius project *)
+(* Clément Blaudeau - Lamp@EPFL 2021 *)
+(** This file defines all the basic structures (as inductive types) of the project. *)
+Require Import Coq.Lists.List Psatz Ensembles.
+Import ListNotations.
+From Celsius Require Export Tactics.
+
+(** * Language structures *)
+
+(** ** Basic types *)
+Definition Var : Type := nat.
+Definition Mtd : Type := nat.
+Definition ClN : Type := nat.
+Definition Loc : Type := nat.
+
+
+(** ** Expression constructors *)
+Inductive Expr: Type :=
+| var   : Var -> Expr
+| this
+| fld   : Expr -> Var -> Expr
+| mtd   : Expr -> Mtd -> (list Expr) -> Expr
+| new   : ClN -> (list Expr) -> Expr
+| asgn  : Expr -> Var -> Expr -> Expr -> Expr.
+
+Inductive Mode: Type :=
+| hot
+| warm
+| cool : nat -> Mode
+| cold.
+Notation "'@' u " := (u:Mode) (at level 20).
+
+Definition Tpe : Type := ClN * Mode.
+
+Inductive Field: Type :=
+| field(type: Tpe)(expr: Expr).
+
+Inductive Method: Type :=
+| method(μ: Mode)(args: list Tpe)(out_type: Tpe)(body: Expr).
+
+Inductive Class: Type :=
+| class(args: list Tpe)(fields: list Field)(methods: Mtd -> (option Method)).
+
+Inductive Program: Type :=
+| program(C: list Class)(entry: Expr).
+
+
+(** ** Constructs *)
+Definition Value : Type := Loc.
+Definition ClassTable: Type := (ClN -> option Class).
+Definition Env: Type   := list Value.
+Definition Obj: Type   := (ClN * Env).
+Definition Store: Type := list Obj.
+Definition StoreTyping : Type := list (Tpe).
+
+Definition LocSet := (Ensemble Loc).
+
+(** ** Global Parameters *)
+Parameter Ξ: list Class.
+Parameter entry: ClN.
+Definition ct: ClassTable := nth_error Ξ.
+Definition main: Mtd := 0.
+
+(** ** Implicit types *)
+Implicit Type σ : Store.
+Implicit Type l ψ v : Loc.
+Implicit Type L : LocSet.
+Implicit Type Σ ρ : Env.
