src/LocalReasoning.v
@@ -10,41 +10,45 @@ Open Scope nat_scope.
 (** ** Local Reasoning theorem *)
 (** We start with a lemma : *)
 Lemma local_reasoning:
-  forall σ σ' L L',
+  forall (σ σ': Store) (L L': LocSet),
     L ⪽ σ ->
     L' ⪽ σ' ->
     (σ, L) ⋖ (σ', L') ->
     σ ≪ σ' ->
-    σ ⊆ σ' ->
+    σ ⪨ σ' ->
     σ ⪯ σ' ->
-    (σ ⊫ L : hot) ->
-    σ' ⊫ L' : hot.
+    σ  ⊨ L  : hot ->
+    σ' ⊨ L' : hot.
 Proof.
-  intros; intros l' Hl'.
+  intros; intros l' H__l'.
+    unfold dash_colon_, notation_reachability_mode, reachable_hot. intros l ?.
   assert (dom σ <= dom σ') by eauto with pM.
-  destruct (PeanoNat.Nat.lt_ge_cases l' (dom σ)).
-  + (* l ∈ (dom σ) *)
-    eapply partialMonotonicity_warm_monotone; eauto .
-    assert (reachability_set σ L l') by (eapply H1; simpl => //; eexists; eauto).
-    inversion H9; steps.
-    eapply H5; eauto with rch.
+  destruct (PeanoNat.Nat.lt_ge_cases l (dom σ)).
+  + (* l ∈ (dom σ) : the object was already in the store *)
+    eapply pM_warm_monotone; eauto.
+    assert (σ ⊨ L ⇝ l).
+    * eapply H1 ; simpl => //.
+      exists l'; split; eauto with rch.
+    * rch_set.
+      eapply H5; eauto with rch.
   + (* l ∉ (dom σ) *)
-    eapply reachability_dom, H2 in Hl'; intuition.
+    pose proof (reachability_dom _ _ _ H6).
+    destruct (H2 l); eauto with lia.
 Qed.
 
 (* Then the main theorem : *)
 Theorem Local_reasoning:
   forall e σ ρ ψ v σ',
-    ⟦e⟧p(σ, ρ, ψ) --> (v, σ') ->
+    ⟦e⟧(σ, ρ, ψ) --> (v, σ') ->
     wf σ ->
     (codom ρ ∪ {ψ}) ⪽ σ ->
-    (σ ⊫ ((codom ρ) ∪ {ψ}) : hot) ->
+    σ  ⊨ ((codom ρ) ∪ {ψ}) : hot ->
     σ' ⊨ v : hot.
 Proof.
   intros.
-  assert (σ' ⊫ (Singleton Loc v) : hot). {
-    eapply local_reasoning;
+  assert (σ' ⊨ (Singleton Loc v) : hot).
+  + eapply local_reasoning;
       eauto using stk_theorem with pM stk cmpt wf lia.
-    eapply scopability_theorem in H; eauto with pM wf lia; steps. }
-  eapply H3; eauto using In_singleton.
+    eapply scopability_theorem in H; eauto with pM wf lia; steps.
+  + eapply H3; eauto using In_singleton.
 Qed.
