src/TypingDefinitions.v
@@ -1,0 +1,78 @@
+(* Celsius project *)
+(* Clément Blaudeau - LAMP@EPFL 2021 *)
+(** Store typing *)
+
+From Celsius Require Export Typing.
+Require Import Coq.ssr.ssreflect Coq.ssr.ssrbool Coq.Lists.List Coq.micromega.Psatz Ensembles.
+(* Import ListNotations. *)
+(* Open Scope nat_scope. *)
+
+
+(** * Main definitions *)
+(** ** Store_typing *)
+(** Here is the link between the abstract environment of types and the store used in execution *)
+Definition store_typing (Σ: StoreTyping) (σ: Store) :=
+  forall l, l < dom Σ -> (exists C ω μ, getObj σ l = Some (C,ω) /\ getType Σ l = Some (C, μ)).
+
+Notation "Σ ⊨ σ" := (store_typing Σ σ) (at level 60, σ at level 98).
+
+(** ** Monotonicity *)
+Definition monotonicity Σ1 Σ2 :=
+  forall l, l < dom Σ1 -> (exists T1 T2, getType Σ1 l = Some T1 /\ getType Σ2 l = Some T2 /\ T1 <: T2).
+Notation "Σ1 ≼ Σ2" := (monotonicity Σ1 Σ2) (at level 60).
+
+Lemma monotonicity_dom :
+  forall Σ1 Σ2, Σ1 ≼ Σ2 -> dom Σ1 <= dom Σ2.
+Proof.
+  intros.
+  edestruct PeanoNat.Nat.le_gt_cases; eauto.
+  destruct (dom Σ1) eqn:E; steps; try lia.
+  specialize (H n).
+  destruct H; try lia; steps.
+  pose proof (nth_error_None Σ2 n).
+  unfold getType in *.
+  eapply_anywhere le_S_n.
+  rewrite_any. exfalso. steps.
+Qed.
+
+Global Hint Resolve monotonicity_dom: typ.
+
+(** ** Authority *)
+Definition authority Σ1 Σ2 :=
+  forall l, l < dom Σ1 -> (exists T, getType Σ1 l = Some T /\ getType Σ2 l = Some T).
+Notation "Σ1 ▷ Σ2" := (monotonicity Σ1 Σ2) (at level 60).
+
+(** ** Value typing (with variants) *)
+
+Inductive value_typing : StoreTyping -> Loc -> Tpe -> Prop :=
+| vt_sub : forall Σ l (T1 T2: Tpe),
+    getType Σ l = Some T1 ->
+    (T1 <: T2) -> value_typing Σ l T2.
+Global Instance notation_value_typing_Tpe : notation_dash_colon StoreTyping Loc Tpe :=
+  { dash_colon_ := value_typing }.
+Global Hint Unfold notation_value_typing_Tpe: notations.
+
+Definition value_typing_mode Σ l μ :=
+  exists C, Σ ⊨ l : (C, μ).
+Global Instance notation_value_typing_Mode : notation_dash_colon StoreTyping Loc Mode :=
+  { dash_colon_ := value_typing_mode }.
+Global Hint Unfold notation_value_typing_Mode: notations.
+
+Definition value_typing_cln Σ l C :=
+  exists μ, Σ ⊨ l : (C, μ).
+Global Instance notation_value_typing_ClN : notation_dash_colon StoreTyping Loc ClN :=
+  { dash_colon_ := value_typing_cln }.
+Global Hint Unfold notation_value_typing_ClN: notations.
+
+Definition value_typing_locset Σ L (μ:Mode) :=
+  forall (l: Loc), (In Loc L l) -> Σ ⊨ l : μ.
+Global Instance notation_value_typing_LocSet : notation_dash_colon StoreTyping LocSet Mode :=
+  { dash_colon_ := value_typing_locset }.
+Global Hint Unfold notation_value_typing_LocSet: notations.
+
+(** ** Stackability *)
+Definition stackability (Σ1 Σ2: StoreTyping) :=
+  forall l, l < dom Σ2 -> (Σ2 ⊨ l : warm) \/ (l < dom Σ1).
+Global Instance notation_stackability_StoreTyping : notation_stackability StoreTyping :=
+  { stackability_ := stackability }.
+From Celsius Require Import Stackability.
